Launchbury/ArityAnalysisImpl.thy
@@ -74,7 +74,7 @@ next
   
   note this[simp] Let(1,2)[simp]
 
-  have "Aexp (Terms.Let \<Gamma> e)[y::=x]\<cdot>n \<sqsubseteq> Afix \<Gamma>[y::h=x]\<cdot>(Aexp e[y::=x]\<cdot>n \<squnion> thunks_AE \<Gamma>[y::h=x]) f|` ( - domA \<Gamma>)" by (simp add: fresh_star_Pair)
+  have "Aexp (Let \<Gamma> e)[y::=x]\<cdot>n \<sqsubseteq> Afix \<Gamma>[y::h=x]\<cdot>(Aexp e[y::=x]\<cdot>n \<squnion> thunks_AE \<Gamma>[y::h=x]) f|` ( - domA \<Gamma>)" by (simp add: fresh_star_Pair)
   also have "(Aexp e[y::=x]\<cdot>n) \<sqsubseteq> (Aexp e\<cdot>n)(y := \<bottom>, x := up\<cdot>0)" by fact
   also have "thunks_AE \<Gamma>[y::h=x] \<sqsubseteq> (thunks_AE \<Gamma>)(y := \<bottom>, x := up\<cdot>0)" by (rule thunks_AE_subst_approx[OF `y \<notin> domA \<Gamma>`])
   also have "(Aexp e\<cdot>n)(y := \<bottom>, x := up\<cdot>0) \<squnion> (thunks_AE \<Gamma>)(y := \<bottom>, x := up\<cdot>0) = (Aexp e\<cdot>n \<squnion> thunks_AE \<Gamma>)(y := \<bottom>, x := up\<cdot>0)" by simp
