ROOT
@@ -44,6 +44,7 @@ session Arity (AFP) in "Launchbury" = "HOLCF-Nominal2" +
     "RedsImprovesArityAnalysis"
     "NoCardinalityAnalysis"
     "FTreeCardinality"
+    "CoCallImplCorrect"
 
 session Nominal2013_1 in "Nominal2-Isabelle2013-1/Nominal" = HOL +
   theories
